add finite In Problem: the function will not be inj anymore... check is necessary

untimed/NewSpfStep.thy
@@ -40,7 +40,7 @@ qed
 thm inv_def
 (* Returns the SPF that switches depending on input.  (spfStep_h1 In Out\<cdot>h)\<cdot>(sbHdElem\<cdot>sb) computes the SPF which has to be applied to the input sb*)
 definition spfStep_inj :: "channel set \<Rightarrow> channel set \<Rightarrow> ('m::message sbElem \<Rightarrow> 'm SPF) \<rightarrow> 'm SB \<rightarrow>'m SPF" where
-"spfStep_inj In Out \<equiv> (\<Lambda> h. (\<Lambda> sb. (if (sbHdElemWell sb) then ufRestrict In Out\<cdot>(h (Abs_sbElem(inv convDiscrUp (sbHdElem\<cdot>sb)))) else ufLeast In Out)))"
+"spfStep_inj In Out \<equiv> (\<Lambda> h. (\<Lambda> sb. (if (sbHdElemWell sb \<and> ubDom\<cdot>sb = In) then ufRestrict In Out\<cdot>(h (Abs_sbElem(inv convDiscrUp (sbHdElem\<cdot>sb)))) else ufLeast In Out)))"
 
 (*inj_on*)
 
@@ -307,28 +307,53 @@ lemma sbhdelemwell_lub_n_exI:assumes "chain Y" and "ubDom\<cdot>(Y i) = In" and 
   shows "\<exists> i. sbHdElemWell (Y i)"
   using assms(1) assms(2) assms(3) assms(4) sbhdelemwell_neg_adm_fin by fastforce
 
+lemma spfStep_inj_mono_h2[simp]:"monofun (\<lambda> sb. (if (sbHdElemWell sb \<and> ubDom\<cdot>sb = In) then ufRestrict In Out\<cdot>(h (Abs_sbElem(inv convDiscrUp (sbHdElem\<cdot>sb)))) else ufLeast In Out))"
+proof(rule monofunI)
+  fix x y::"'a stream\<^sup>\<Omega>"
+  assume a1:"x \<sqsubseteq> y"
+  show "(if sbHdElemWell x \<and> ubDom\<cdot>x = In then ufRestrict In Out\<cdot>(h (Abs_sbElem (inv convDiscrUp (sbHdElem\<cdot>x)))) else ufLeast In Out) \<sqsubseteq>
+       (if sbHdElemWell y \<and> ubDom\<cdot>y = In then ufRestrict In Out\<cdot>(h (Abs_sbElem (inv convDiscrUp (sbHdElem\<cdot>y)))) else ufLeast In Out)"
+  proof(cases "sbHdElemWell x \<and> ubDom\<cdot>x = In")
+    case True
+    then have true_y:"sbHdElemWell y"
+      by (metis a1 bottomI ubdom_below ubgetch_below sbHdElemWell_def)
+    have a3:"sbHdElem\<cdot>x = sbHdElem\<cdot>y"
+        apply(rule sbHdElem_eq)
+        apply (meson True sbHdElemWell_def) 
+        using True a1 by blast
+    have "ufRestrict In Out\<cdot>(h (Abs_sbElem (inv convDiscrUp (sbHdElem\<cdot>x)))) \<sqsubseteq> ufRestrict In Out\<cdot>(h (Abs_sbElem (inv convDiscrUp (sbHdElem\<cdot>y))))"
+        by (smt a1 a3 below_option_def po_eq_conv spfrt_step ufun_rel_eq)
+      then show ?thesis
+        using a1 true_y ubdom_below by auto
+  next
+    case False
+    then show ?thesis
+      by auto
+  qed
+qed
 
-lemma spfStep_inj_cont_h[simp]:"cont (\<lambda> sb. (if (sbHdElemWell sb) then ufRestrict In Out\<cdot>(h (Abs_sbElem(inv convDiscrUp (sbHdElem\<cdot>sb)))) else ufLeast In Out))"(*Maybe In has to be finite for cont*)
+lemma spfStep_inj_cont_h[simp]:assumes "finite In" 
+  shows "cont (\<lambda> sb. (if (sbHdElemWell sb \<and> ubDom\<cdot>sb = In) then ufRestrict In Out\<cdot>(h (Abs_sbElem(inv convDiscrUp (sbHdElem\<cdot>sb)))) else ufLeast In Out))"(*Maybe In has to be finite for cont*)
 proof(rule Cont.contI2, simp)
   fix Y::"nat \<Rightarrow> 'a stream\<^sup>\<Omega>"
   assume a1:"chain Y"
-  assume a2:"chain (\<lambda>i. if sbHdElemWell (Y i) then ufRestrict In Out\<cdot>(h (Abs_sbElem (inv convDiscrUp (sbHdElem\<cdot>(Y i))))) else ufLeast In Out)"
-  have dom:"ufDom\<cdot>(\<Squnion>i::nat. if sbHdElemWell (Y i) then ufRestrict In Out\<cdot>(h (Abs_sbElem (inv convDiscrUp (sbHdElem\<cdot>(Y i))))) else ufLeast In Out) = In"
+  assume a2:"chain (\<lambda>i. if sbHdElemWell (Y i) \<and> ubDom\<cdot>(Y i) = In then ufRestrict In Out\<cdot>(h (Abs_sbElem (inv convDiscrUp (sbHdElem\<cdot>(Y i))))) else ufLeast In Out)"
+  have dom:"ufDom\<cdot>(\<Squnion>i::nat. if sbHdElemWell (Y i) \<and> ubDom\<cdot>(Y i) = In then ufRestrict In Out\<cdot>(h (Abs_sbElem (inv convDiscrUp (sbHdElem\<cdot>(Y i))))) else ufLeast In Out) = In"
     by (smt a2 ufRestrict_dom ufdom_lub_eq ufleast_ufdom)
-  have ran:"ufRan\<cdot>(\<Squnion>i::nat. if sbHdElemWell (Y i) then ufRestrict In Out\<cdot>(h (Abs_sbElem (inv convDiscrUp (sbHdElem\<cdot>(Y i))))) else ufLeast In Out) = Out"
+  have ran:"ufRan\<cdot>(\<Squnion>i::nat. if sbHdElemWell (Y i) \<and> ubDom\<cdot>(Y i) = In then ufRestrict In Out\<cdot>(h (Abs_sbElem (inv convDiscrUp (sbHdElem\<cdot>(Y i))))) else ufLeast In Out) = Out"
     by (smt a2 ufRestrict_ran ufleast_ufRan ufran_lub_eq)  
   have sbHdEq:"\<And>i. sbHdElemWell (Y i) \<Longrightarrow> (Abs_sbElem (inv convDiscrUp (sbHdElem\<cdot>(\<Squnion>i. Y i)))) = (Abs_sbElem (inv convDiscrUp (sbHdElem\<cdot>(Y i))))"
     by (metis a1 is_ub_thelub sbHdElemWell_def sbHdElem_eq)
-  show "(if sbHdElemWell (\<Squnion>i. Y i) then ufRestrict In Out\<cdot>(h (Abs_sbElem (inv convDiscrUp (sbHdElem\<cdot>(\<Squnion>i. Y i))))) else ufLeast In Out) \<sqsubseteq>
-       (\<Squnion>i. if sbHdElemWell (Y i) then ufRestrict In Out\<cdot>(h (Abs_sbElem (inv convDiscrUp (sbHdElem\<cdot>(Y i))))) else ufLeast In Out)"
-  proof(cases "sbHdElemWell (\<Squnion>i. Y i)")
+  show "(if sbHdElemWell (\<Squnion>i::nat. Y i) \<and> ubDom\<cdot>(\<Squnion>i::nat. Y i) = In then ufRestrict In Out\<cdot>(h (Abs_sbElem (inv convDiscrUp (sbHdElem\<cdot>(\<Squnion>i. Y i))))) else ufLeast In Out) \<sqsubseteq>
+       (\<Squnion>i. if sbHdElemWell (Y i) \<and> ubDom\<cdot>(Y i) = In then ufRestrict In Out\<cdot>(h (Abs_sbElem (inv convDiscrUp (sbHdElem\<cdot>(Y i))))) else ufLeast In Out)"
+  proof(cases "sbHdElemWell (\<Squnion>i::nat. Y i) \<and> ubDom\<cdot>(\<Squnion>i::nat. Y i) = In")
     case True
     obtain n where n_def:"sbHdElemWell (Y n)"
-      sorry
-    then have h1:"(if sbHdElemWell (\<Squnion>i. Y i) then ufRestrict In Out\<cdot>(h (Abs_sbElem (inv convDiscrUp (sbHdElem\<cdot>(\<Squnion>i. Y i))))) else ufLeast In Out) = (ufRestrict In Out\<cdot>(h (Abs_sbElem (inv convDiscrUp (sbHdElem\<cdot>( Y n))))))"
+      using True a1 assms sbhdelemwell_neg_adm_fin by auto
+    then have h1:"(if sbHdElemWell (\<Squnion>i. Y i) \<and> ubDom\<cdot>(\<Squnion>i::nat. Y i) = In then ufRestrict In Out\<cdot>(h (Abs_sbElem (inv convDiscrUp (sbHdElem\<cdot>(\<Squnion>i. Y i))))) else ufLeast In Out) = (ufRestrict In Out\<cdot>(h (Abs_sbElem (inv convDiscrUp (sbHdElem\<cdot>( Y n))))))"
       by(subst sbHdEq[of n], simp_all add: True n_def)
-    then have h2:"ufRestrict In Out\<cdot>(h (Abs_sbElem (inv convDiscrUp (sbHdElem\<cdot>(Y n)))))\<sqsubseteq> (\<Squnion>i. (if sbHdElemWell (Y i) then ufRestrict In Out\<cdot>(h (Abs_sbElem (inv convDiscrUp (sbHdElem\<cdot>(Y i))))) else ufLeast In Out))"
-        using a2 below_lub n_def by fastforce
+    then have h2:"ufRestrict In Out\<cdot>(h (Abs_sbElem (inv convDiscrUp (sbHdElem\<cdot>(Y n)))))\<sqsubseteq> (\<Squnion>i. (if sbHdElemWell (Y i) \<and> ubDom\<cdot>(Y i) = In then ufRestrict In Out\<cdot>(h (Abs_sbElem (inv convDiscrUp (sbHdElem\<cdot>(Y i))))) else ufLeast In Out))"
+      by (smt a1 a2 below_lub n_def po_class.chain_def ubdom_chain_eq2)
     then show ?thesis
       by (simp add: h1)
   next
@@ -338,80 +363,178 @@ proof(rule Cont.contI2, simp)
   qed
 qed
   
-lemma spfStep_inj_mono[simp]:"monofun (\<lambda> h. (\<Lambda> sb. (if (sbHdElemWell sb) then ufRestrict In Out\<cdot>(h (Abs_sbElem(inv convDiscrUp (sbHdElem\<cdot>sb)))) else ufLeast In Out)))"
-proof(rule monofunI)
-  fix x y ::"'a sbElem \<Rightarrow> 'b ufun"
-  assume a1:"x \<sqsubseteq> y"
-  show "(\<Lambda> sb. if sbHdElemWell sb then ufRestrict In Out\<cdot>(x (Abs_sbElem (inv convDiscrUp (sbHdElem\<cdot>sb)))) else ufLeast In Out) \<sqsubseteq>
-       (\<Lambda> sb. if sbHdElemWell sb then ufRestrict In Out\<cdot>(y (Abs_sbElem (inv convDiscrUp (sbHdElem\<cdot>sb)))) else ufLeast In Out)"
-  proof(rule cfun_belowI,auto)
-    fix xa::"'a stream\<^sup>\<Omega>"
-    assume a2:"sbHdElemWell xa"
-    show "ufRestrict In Out\<cdot>(x (Abs_sbElem (inv convDiscrUp (sbHdElem\<cdot>xa)))) \<sqsubseteq> ufRestrict In Out\<cdot>(y (Abs_sbElem (inv convDiscrUp (sbHdElem\<cdot>xa))))"
-      by (simp add: a1 cont_pref_eq1I fun_belowD)
-  qed
-qed
+lemma spfStep_inj_mono[simp]:assumes "finite In" 
+  shows "monofun (\<lambda> h. (\<Lambda> sb. (if (sbHdElemWell sb \<and> ubDom\<cdot>sb = In) then ufRestrict In Out\<cdot>(h (Abs_sbElem(inv convDiscrUp (sbHdElem\<cdot>sb)))) else ufLeast In Out)))"
+  apply (rule monofunI)
+  apply (rule cfun_belowI)
+  apply (simp add: assms)
+  apply auto
+  by (simp add: fun_belowD monofun_cfun_arg)
     
 
-lemma spfStep_inj_cont[simp]:"cont (\<lambda> h. (\<Lambda> sb. (if (sbHdElemWell sb) then ufRestrict In Out\<cdot>(h (Abs_sbElem(inv convDiscrUp (sbHdElem\<cdot>sb)))) else ufLeast In Out)))"
-proof(rule Cont.contI2, simp)
+lemma spfStep_inj_cont[simp]: assumes "finite In"
+  shows "cont (\<lambda> h. (\<Lambda> sb. (if (sbHdElemWell sb \<and> ubDom\<cdot>sb = In)
+             then ufRestrict In Out\<cdot>(h (Abs_sbElem(inv convDiscrUp (sbHdElem\<cdot>sb)))) else ufLeast In Out)))"
+proof (rule Cont.contI2, simp add: assms)
   fix Y::"nat \<Rightarrow> 'a sbElem \<Rightarrow> 'b ufun"
-  assume a1: "chain Y"
-  assume a2: "chain (\<lambda>i::nat. \<Lambda> (sb::'a stream\<^sup>\<Omega>). if sbHdElemWell sb then ufRestrict In Out\<cdot>(Y i (Abs_sbElem (inv convDiscrUp (sbHdElem\<cdot>sb)))) else ufLeast In Out)"
-  have cont_lub:"\<And>x::'a stream\<^sup>\<Omega>. cont (\<lambda>x::'a stream\<^sup>\<Omega>. \<Squnion>i::nat. if sbHdElemWell x then ufRestrict In Out\<cdot>(Y i (Abs_sbElem (inv convDiscrUp (sbHdElem\<cdot>x)))) else ufLeast In Out)"
-  proof(rule cont2cont_lub, simp_all add: a2)
-    fix sb::"'a stream\<^sup>\<Omega>"
-    show "chain (\<lambda>i. if sbHdElemWell sb then ufRestrict In Out\<cdot>(Y i (Abs_sbElem (inv convDiscrUp (sbHdElem\<cdot>sb)))) else ufLeast In Out)"
-    proof(cases "sbHdElemWell sb")
-      case True
-      then show ?thesis 
-        by (simp add: a1 ch2ch_fun)
-    next
-      case False
-      then show ?thesis
-        by simp
-    qed
+  assume a1: " chain Y"
+  assume a2: "chain (\<lambda>i::nat. \<Lambda> (sb::'a stream\<^sup>\<Omega>).
+                          if sbHdElemWell sb \<and> ubDom\<cdot>sb = In
+                          then ufRestrict In Out\<cdot>(Y i (Abs_sbElem (inv convDiscrUp (sbHdElem\<cdot>sb)))) else ufLeast In Out)"
+  have cont_lub: " \<And>x::'a stream\<^sup>\<Omega>.
+       cont (\<lambda>x::'a stream\<^sup>\<Omega>.
+                \<Squnion>i::nat.
+                   if sbHdElemWell x \<and> ubDom\<cdot>x = In then ufRestrict In Out\<cdot>(Y i (Abs_sbElem (inv convDiscrUp (sbHdElem\<cdot>x))))
+                   else ufLeast In Out)"
+    proof (rule cont2cont_lub, simp_all add: assms)
+    fix xa :: "'a stream\<^sup>\<Omega>"
+    have f1: "\<forall>n. Y n \<sqsubseteq> Y (Suc n)"
+      by (meson a1 po_class.chain_def)
+    obtain nn :: "(nat \<Rightarrow> 'b ufun) \<Rightarrow> nat" where
+      f2: "\<forall>f. (\<not> chain f \<or> (\<forall>n. f n \<sqsubseteq> f (Suc n))) \<and> (chain f \<or> f (nn f) \<notsqsubseteq> f (Suc (nn f)))"
+      using po_class.chain_def by moura
+    have "(if sbHdElemWell xa \<and> ubDom\<cdot>xa = In then ufRestrict In Out\<cdot> (Y (nn (\<lambda>n. if sbHdElemWell xa \<and> ubDom\<cdot>xa = In then ufRestrict In Out\<cdot> (Y n (Abs_sbElem (inv convDiscrUp (sbHdElem\<cdot>xa)))) else ufLeast In Out)) (Abs_sbElem (inv convDiscrUp (sbHdElem\<cdot>xa)))) else ufLeast In Out) \<sqsubseteq> (if sbHdElemWell xa \<and> ubDom\<cdot>xa = In then ufRestrict In Out\<cdot> (Y (Suc (nn (\<lambda>n. if sbHdElemWell xa \<and> ubDom\<cdot>xa = In then ufRestrict In Out\<cdot> (Y n (Abs_sbElem (inv convDiscrUp (sbHdElem\<cdot>xa)))) else ufLeast In Out))) (Abs_sbElem (inv convDiscrUp (sbHdElem\<cdot>xa)))) else ufLeast In Out)"
+      using f1 by (simp add: cont_pref_eq1I fun_belowD)
+    then show "chain (\<lambda>n. if sbHdElemWell xa \<and> ubDom\<cdot>xa = In then ufRestrict In Out\<cdot> (Y n (Abs_sbElem (inv convDiscrUp (sbHdElem\<cdot>xa)))) else ufLeast In Out)"
+      using f2 by meson
   qed
-  show "(\<Lambda> sb. if sbHdElemWell sb then ufRestrict In Out\<cdot>((\<Squnion>i::nat. Y i) (Abs_sbElem (inv convDiscrUp (sbHdElem\<cdot>sb)))) else ufLeast In Out) \<sqsubseteq>
-       (\<Squnion>i. \<Lambda> sb. if sbHdElemWell sb then ufRestrict In Out\<cdot>(Y i (Abs_sbElem (inv convDiscrUp (sbHdElem\<cdot>sb)))) else ufLeast In Out)"
-    apply(subst lub_cfun, simp add: a2)
-    apply(simp only: below_cfun_def below_fun_def)
-    apply(subst beta_cfun, simp)
+  show "(\<Lambda> (sb::'a stream\<^sup>\<Omega>).
+           if sbHdElemWell sb \<and> ubDom\<cdot>sb = In
+           then ufRestrict In Out\<cdot>((\<Squnion>i::nat. Y i) (Abs_sbElem (inv convDiscrUp (sbHdElem\<cdot>sb)))) else ufLeast In Out) \<sqsubseteq>
+       (\<Squnion>i::nat.
+           \<Lambda> (sb::'a stream\<^sup>\<Omega>).
+              if sbHdElemWell sb \<and> ubDom\<cdot>sb = In then ufRestrict In Out\<cdot>(Y i (Abs_sbElem (inv convDiscrUp (sbHdElem\<cdot>sb))))
+              else ufLeast In Out)"
+  apply(subst lub_cfun, simp add: a2)
+  apply(simp only: below_cfun_def below_fun_def)
+  apply(subst beta_cfun, simp add: assms)
+    apply(subst beta_cfun, simp add: assms)
     apply(subst beta_cfun)
-    apply simp
-    apply(subst beta_cfun, simp only: cont_lub)
+    using cont_lub apply blast
     by (simp add: a1 ch2ch_fun cont2contlubE lub_fun)
 qed
+
   
-        
-    
-lemma sbElem_surj_h:" \<exists>sb. f = (inv convDiscrUp (sbHdElem\<cdot>sb)) \<and> sbHdElemWell sb"
-proof-    
-  show "\<exists>sb. f = inv convDiscrUp (sbHdElem\<cdot>sb) \<and> sbHdElemWell sb"
-    sorry
+thm Rep_sbElem_inverse
+
+(*
+definition convSB :: "(channel \<rightharpoonup> 'm discr\<^sub>\<bottom>) \<Rightarrow> 'm stream ubundle" where
+"convSB sb \<equiv> Abs_ubundle (\<lambda>c. (c \<in> dom sb) \<leadsto> (lscons\<cdot>(sb \<rightharpoonup> c)\<cdot>\<epsilon>))"
+*)
+
+lemma bla: assumes "sbElemWell (sb)" shows "ubWell (\<lambda>c. (c \<in> dom sb) \<leadsto> (lscons\<cdot>((convDiscrUp sb) \<rightharpoonup> c)\<cdot>\<epsilon>))"
+  apply (rule ubwellI) 
+  apply (simp add: domIff2)
+  unfolding usclOkay_stream_def
+proof - 
+  fix c
+  assume c_in_dom: "c \<in> dom sb"
+  have f0: "sb\<rightharpoonup>c \<in> ctype c"
+    by (simp add: assms c_in_dom sbElemWellI)
+  have f1: "updis(sb\<rightharpoonup>c) && \<epsilon> = convDiscrUp sb\<rightharpoonup>c && \<epsilon>"
+    by (simp add: c_in_dom convDiscrUp_def up_def)
+  have f2: "updis(sb\<rightharpoonup>c) && \<epsilon> = \<up>(sb\<rightharpoonup>c)"
+    by (simp add: sup'_def)
+  have f3: "sdom\<cdot>(convDiscrUp sb\<rightharpoonup>c && \<epsilon>) = sdom\<cdot>(\<up>sb\<rightharpoonup>c)"
+    using f1 f2 by auto
+  have f4: "sdom\<cdot>(\<up>sb\<rightharpoonup>c) = {sb\<rightharpoonup>c}"
+    by simp
+  show "sdom\<cdot>(convDiscrUp sb\<rightharpoonup>c && \<epsilon>) \<subseteq> ctype c"
+    by (simp add: f0 f3)
 qed
-          
-lemma sbElem_surj:"\<exists>sb. sbE =  Abs_sbElem (inv convDiscrUp (sbHdElem\<cdot>sb)) \<and> sbHdElemWell sb"
-  sorry
+
+lemma bla_dom: assumes "sbElemWell (sb)" shows "ubDom\<cdot>(convSB (convDiscrUp sb)) = dom sb"
+  apply (simp add: convSB_def)
+  apply (subst ubdom_ubrep_eq)
+   apply (simp add: assms bla)
+  by simp
+
+lemma bla_apply: assumes "sbElemWell (sb)" and "c \<in> dom sb" 
+  shows " (convSB (convDiscrUp sb)) . c = \<up>(sb \<rightharpoonup>c)"
+  apply (simp add: convSB_def)
+  apply (simp add: ubgetch_ubrep_eq assms bla)
+  by (simp add: assms(2) convDiscrUp_def sup'_def up_def)
+
+lemma sbElem_surj:
+  shows "\<And> sbE. \<exists>sb. sbE =  Abs_sbElem (inv convDiscrUp (sbHdElem\<cdot>sb)) 
+                    \<and> sbHdElemWell sb \<and> ubDom\<cdot>sb = dom (Rep_sbElem sbE)"
+proof -
+  fix sbE ::"'a sbElem"
+  obtain daFun where daFun_def: "daFun  = Rep_sbElem sbE"
+    by (metis Rep_sbElem_inverse)
+  have f0: "sbElemWell (Rep_sbElem sbE)"
+    using Rep_sbElem by auto
+  have f1: "sbElemWell daFun"
+    by (simp add: daFun_def f0)
+  have f2: "\<forall>c\<in> dom daFun. daFun\<rightharpoonup>c \<in> ctype c"
+    using f1 sbElemWell_def by auto
+  have f3: "dom daFun = dom (Rep_sbElem sbE)"
+    by (simp add: daFun_def)
+  obtain daBundle where daBundle_def: "daBundle = convSB (convDiscrUp daFun)"
+    by simp
+  have daDom_eq: "ubDom\<cdot>daBundle = dom daFun"
+    apply (simp add: daBundle_def)
+    by (simp add: f1 bla_dom)
+  have daBundle_elem_wel: "sbHdElemWell daBundle"
+    apply (simp add: sbHdElemWell_def)
+  proof rule
+    fix c::channel
+    assume c_in_dom: "c \<in> ubDom\<cdot>daBundle"
+    have c_in_dom_2: "c \<in> dom daFun"
+      using c_in_dom daDom_eq by auto
+
+    show "daBundle  .  c \<noteq> \<epsilon>"
+      apply (simp add: daBundle_def)
+      by (simp add: bla_apply f1 c_in_dom_2)
+  qed    
+  have f111: "sbHdElem\<cdot>daBundle = convDiscrUp daFun"
+    apply (simp add: daBundle_def)
+    apply (simp add: sbHdElem_cont sbHdElem_def)
+    apply (rule part_eq)
+    using daBundle_def daDom_eq apply auto[1]
+    apply simp
+    apply (subst add: daFun_def)
+    apply (subst convSB_def)
+    apply (subst ubgetch_ubrep_eq)
+    apply (simp add: bla f1)
+    apply simp
+    using daBundle_def daDom_eq by auto
+  show "\<exists>sb. sbE =  Abs_sbElem (inv convDiscrUp (sbHdElem\<cdot>sb)) 
+    \<and> sbHdElemWell sb \<and> ubDom\<cdot>sb = dom (Rep_sbElem sbE)"
+    apply (rule_tac x="daBundle" in exI)
+    apply rule defer
+     apply (simp add: daBundle_elem_wel daDom_eq f3)
+    apply (subst f111)
+    by (simp add: Rep_sbElem_inverse convDiscrUp_inj daFun_def)
+qed
     
-lemma spfStep_inj_on[simp]:"inj_on (Rep_cfun (spfStep_inj In Out)) {h. \<forall>m. ufDom\<cdot>(h m) = In \<and> ufRan\<cdot>(h m) = Out}"
-proof(simp add: spfStep_inj_def, rule inj_onI)
+lemma spfStep_inj_on[simp]:assumes "finite In" shows "inj_on (Rep_cfun (spfStep_inj In Out)) {h. \<forall>m. ufDom\<cdot>(h m) = In \<and> ufRan\<cdot>(h m) = Out}"
+proof (simp add: spfStep_inj_def, rule inj_onI)
   fix x y :: "'a sbElem \<Rightarrow> ('a stream\<^sup>\<Omega>) ufun"
   assume ax:" x \<in> {h. \<forall>m. ufDom\<cdot>(h m) = In \<and> ufRan\<cdot>(h m) = Out}"
   assume ay:" y \<in> {h. \<forall>m. ufDom\<cdot>(h m) = In \<and> ufRan\<cdot>(h m) = Out}"
-  assume a1:"(\<Lambda> sb. if sbHdElemWell sb then ufRestrict In Out\<cdot>(x (Abs_sbElem (inv convDiscrUp (sbHdElem\<cdot>sb)))) else ufLeast In Out) =
-             (\<Lambda> sb. if sbHdElemWell sb then ufRestrict In Out\<cdot>(y (Abs_sbElem (inv convDiscrUp (sbHdElem\<cdot>sb)))) else ufLeast In Out)"
-  have ya:"(\<forall>elem.  ufDom\<cdot>(y elem) = In \<and> ufRan\<cdot>(y elem) = Out)"
-    using ay by auto
-  have xa:"(\<forall>elem.  ufDom\<cdot>(x elem) = In \<and> ufRan\<cdot>(x elem) = Out)"
-    using ax by auto
+  assume a1:"
+       (\<Lambda> (h::'a sbElem \<Rightarrow> ('a stream\<^sup>\<Omega>) ufun) (sb::'a stream\<^sup>\<Omega>). if sbHdElemWell sb \<and> ubDom\<cdot>sb = In then ufRestrict In Out\<cdot>(h (Abs_sbElem (inv convDiscrUp (sbHdElem\<cdot>sb)))) else ufLeast In Out)\<cdot>x =
+       (\<Lambda> (h::'a sbElem \<Rightarrow> ('a stream\<^sup>\<Omega>) ufun) (sb::'a stream\<^sup>\<Omega>). if sbHdElemWell sb \<and> ubDom\<cdot>sb = In then ufRestrict In Out\<cdot>(h (Abs_sbElem (inv convDiscrUp (sbHdElem\<cdot>sb)))) else ufLeast In Out)\<cdot>y"  
+  have a2: "(\<Lambda> (h::'a sbElem \<Rightarrow> ('a stream\<^sup>\<Omega>) ufun) (sb::'a stream\<^sup>\<Omega>). if sbHdElemWell sb \<and> ubDom\<cdot>sb = In then ufRestrict In Out\<cdot>(h (Abs_sbElem (inv convDiscrUp (sbHdElem\<cdot>sb)))) else ufLeast In Out)\<cdot>x =
+            (\<Lambda> sb. if sbHdElemWell sb \<and> ubDom\<cdot>sb = In then ufRestrict In Out\<cdot>(x (Abs_sbElem (inv convDiscrUp (sbHdElem\<cdot>sb)))) else ufLeast In Out)"
+    by (simp add: assms)
+  have a3: "(\<Lambda> (h::'a sbElem \<Rightarrow> ('a stream\<^sup>\<Omega>) ufun) (sb::'a stream\<^sup>\<Omega>). if sbHdElemWell sb \<and> ubDom\<cdot>sb = In then ufRestrict In Out\<cdot>(h (Abs_sbElem (inv convDiscrUp (sbHdElem\<cdot>sb)))) else ufLeast In Out)\<cdot>y =
+            (\<Lambda> sb. if sbHdElemWell sb \<and> ubDom\<cdot>sb = In then ufRestrict In Out\<cdot>(y (Abs_sbElem (inv convDiscrUp (sbHdElem\<cdot>sb)))) else ufLeast In Out)"
+    by (simp add: assms)
+  have a4: "(\<Lambda> sb. if sbHdElemWell sb \<and> ubDom\<cdot>sb = In then ufRestrict In Out\<cdot>(x (Abs_sbElem (inv convDiscrUp (sbHdElem\<cdot>sb)))) else ufLeast In Out) = 
+            (\<Lambda> sb. if sbHdElemWell sb \<and> ubDom\<cdot>sb = In then ufRestrict In Out\<cdot>(y (Abs_sbElem (inv convDiscrUp (sbHdElem\<cdot>sb)))) else ufLeast In Out)"
+    using a1 a2 a3 by auto
   show "x = y"
   proof(cases "x \<noteq> y")
     case True
     then obtain sbE where sbE_def:" x sbE \<noteq> y sbE"
       by fastforce
-    then obtain sb where sb_def:"((inv convDiscrUp (sbHdElem\<cdot>sb))) =  (Rep_sbElem sbE) \<and> sbHdElemWell sb"
-      using sbElem_surj_h  by metis
+    have blabla: " dom (Rep_sbElem sbE) = In"
+      sledgehammer
+      sorry
+    then obtain sb where sb_def:"((inv convDiscrUp (sbHdElem\<cdot>sb))) =  (Rep_sbElem sbE) \<and> sbHdElemWell sb \<and> ubDom\<cdot>sb = In"
+      by (metis (full_types) Abs_sbElem_inverse mem_Collect_eq sbElem_surj sbHdElemWell_def sbHdElem_sbElemWell)
     then have spf_uneq:"(x (Abs_sbElem (inv convDiscrUp (sbHdElem\<cdot>sb)))) \<noteq> (y (Abs_sbElem (inv convDiscrUp (sbHdElem\<cdot>sb))))"
       by(simp add: Rep_sbElem_inverse sb_def sbE_def)
     obtain spf1 where spf_1_def:" (x (Abs_sbElem (inv convDiscrUp (sbHdElem\<cdot>sb)))) = spf1"
@@ -419,32 +542,32 @@ proof(simp add: spfStep_inj_def, rule inj_onI)
     obtain spf2 where spf_2_def:" (y (Abs_sbElem (inv convDiscrUp (sbHdElem\<cdot>sb)))) = spf2"
       by simp
     have ufR_uneq:"ufRestrict In Out\<cdot>spf1 \<noteq> ufRestrict In Out\<cdot>spf2"
-      using ax ya spf_uneq spf_1_def spf_2_def by auto
+      by (metis (mono_tags, lifting) Rep_sbElem_inverse ax ay mem_Collect_eq sbE_def sb_def spf_1_def spf_2_def ufRestrict_apply)
     have uf_eq:"ufRestrict In Out\<cdot>spf1 = spf1 \<and> ufRestrict In Out\<cdot>spf2 = spf2"
-      using ax spf_1_def spf_2_def ya by auto
+      using ax ay spf_1_def spf_2_def by auto
     then have "spf1 \<noteq> spf2"
       using ufR_uneq by auto
     have sb_Well:"sbHdElemWell sb"
       by(simp add: sb_def)
-    have h:"(\<lambda> sb. if sbHdElemWell sb then ufRestrict In Out\<cdot>(x (Abs_sbElem (inv convDiscrUp (sbHdElem\<cdot>sb)))) else ufLeast In Out) \<noteq>
-             (\<lambda> sb. if sbHdElemWell sb then ufRestrict In Out\<cdot>(y (Abs_sbElem (inv convDiscrUp (sbHdElem\<cdot>sb)))) else ufLeast In Out)"
+    have h:"(\<lambda> sb. if sbHdElemWell sb \<and> ubDom\<cdot>sb = In then ufRestrict In Out\<cdot>(x (Abs_sbElem (inv convDiscrUp (sbHdElem\<cdot>sb)))) else ufLeast In Out) \<noteq>
+             (\<lambda> sb. if sbHdElemWell sb \<and> ubDom\<cdot>sb = In then ufRestrict In Out\<cdot>(y (Abs_sbElem (inv convDiscrUp (sbHdElem\<cdot>sb)))) else ufLeast In Out)"
       apply(subst fun_eq_iff,auto)
       apply(rule_tac x="sb" in exI)
-      by(simp add: spf_1_def spf_2_def ufR_uneq sb_Well)
-    have "(\<Lambda> sb. if sbHdElemWell sb then ufRestrict In Out\<cdot>(x (Abs_sbElem (inv convDiscrUp (sbHdElem\<cdot>sb)))) else ufLeast In Out) \<noteq>
-             (\<Lambda> sb. if sbHdElemWell sb then ufRestrict In Out\<cdot>(y (Abs_sbElem (inv convDiscrUp (sbHdElem\<cdot>sb)))) else ufLeast In Out)"
+      using sb_def spf_1_def spf_2_def ufR_uneq by blast
+    have "(\<Lambda> sb. if sbHdElemWell sb \<and> ubDom\<cdot>sb = In then ufRestrict In Out\<cdot>(x (Abs_sbElem (inv convDiscrUp (sbHdElem\<cdot>sb)))) else ufLeast In Out) \<noteq>
+             (\<Lambda> sb. if sbHdElemWell sb \<and> ubDom\<cdot>sb = In then ufRestrict In Out\<cdot>(y (Abs_sbElem (inv convDiscrUp (sbHdElem\<cdot>sb)))) else ufLeast In Out)"
       apply(subst cfun_eq_iff, auto)
       apply(rule_tac x="sb" in exI)
-      by(simp add: spf_1_def spf_2_def ufR_uneq sb_Well)
+      using \<open>(spf1::('a stream\<^sup>\<Omega>) ufun) \<noteq> (spf2::('a stream\<^sup>\<Omega>) ufun)\<close> assms sb_def spf_1_def spf_2_def uf_eq by auto
     then show ?thesis
-      by(simp add: a1)
+      by (simp add: a4)
   next
     case False
     then show ?thesis 
       by simp
   qed
 qed
-  
+
 lemma spfStep_eq_sb:assumes"sb1 \<sqsubseteq> sb2" and "sbHdElemWell sb1" shows "spfStep_inj In Out\<cdot>h\<cdot>sb1 = spfStep_inj In Out\<cdot>h\<cdot>sb2"
   sorry
 
@@ -469,7 +592,7 @@ proof(rule spf_contI2)
         by (simp add: a1 cont_pref_eq2I)
       then show "spfStep_inj In Out\<cdot>h\<cdot>x \<rightleftharpoons> x \<sqsubseteq> spfStep_inj In Out\<cdot>h\<cdot>y \<rightleftharpoons> y"
         apply (simp add: below_ufun_def below_cfun_def below_fun_def)
-        by (smt a1 below_option_def below_refl box_below monofun_cfun_arg)
+        by (metis a1 below_option_def below_refl cfun_belowI monofun_cfun)
     qed
   next
     fix Y::"nat \<Rightarrow> 'a stream\<^sup>\<Omega>"
@@ -486,9 +609,12 @@ lemma ufLeast_out_ubDom:assumes "ubDom\<cdot>sb = In" shows "ubDom\<cdot>(ufLeas
   apply(simp add: ufLeast_def assms)
   by (metis assms ubclDom_ubundle_def ubcldom_least_cs)
     
-lemma spfStep_inj_out_dom[simp]:assumes"ubDom\<cdot>sb = In" shows "ubDom\<cdot>(spfStep_inj In Out\<cdot> h \<cdot> f \<rightleftharpoons> sb) = Out"
-  apply(simp add: spfStep_inj_def assms ufLeast_out_ubDom)
-  by (metis assms ubclDom_ubundle_def ufRestrict_dom ufRestrict_ran ufran_2_ubcldom2)
+lemma spfStep_inj_out_dom[simp]:assumes"ubDom\<cdot>sb = In" and "finite In" shows "ubclDom\<cdot>(spfStep_inj In Out\<cdot> h \<cdot> f \<rightleftharpoons> sb) = Out"
+  apply (subst ufran_2_ubcldom2)
+   apply (simp add: spfStep_inj_def assms)
+   apply (simp add: assms(1) ubclDom_ubundle_def)
+  by (simp add: assms(2) spfStep_inj_def)
+(*  by (metis assms ubclDom_ubundle_def ufRestrict_dom ufRestrict_ran ufran_2_ubcldom2) *)
 
 lemma spfStep_inj_ran[simp]:assumes "finite In" shows"ufRan\<cdot>(spfStep_inj In Out\<cdot> h \<cdot> f) = Out"
   by(simp add: spfStep_inj_def assms)
@@ -497,7 +623,7 @@ lemma spf_pref_eq_2: assumes "(f \<sqsubseteq> g)"
   shows "(f \<rightleftharpoons> a) \<sqsubseteq> (g \<rightleftharpoons> a)" 
   by (metis assms below_ufun_def below_option_def cfun_below_iff po_eq_conv)
     
-lemma spfStep_inj_inner_well[simp]:"ufWell(\<Lambda> sb. (ubDom\<cdot>sb = In) \<leadsto> spfStep_inj In Out\<cdot>h\<cdot>sb \<rightleftharpoons> sb)"
+lemma spfStep_inj_inner_well[simp]:assumes "finite In" shows  "ufWell(\<Lambda> sb. (ubDom\<cdot>sb = In) \<leadsto> spfStep_inj In Out\<cdot>h\<cdot>sb \<rightleftharpoons> sb)"
   proof(rule ufwellI)
     fix b::"'a SB"
     assume "b \<in> dom (Rep_cfun (\<Lambda> sb. (ubDom\<cdot>sb = In)\<leadsto>spfStep_inj In Out\<cdot>h\<cdot>sb \<rightleftharpoons> sb))"
@@ -509,7 +635,12 @@ lemma spfStep_inj_inner_well[simp]:"ufWell(\<Lambda> sb. (ubDom\<cdot>sb = In) \
         by (smt b_def domIff)
     qed
     thus "ubDom\<cdot>(the ((\<Lambda> sb. (ubDom\<cdot>sb = In)\<leadsto>spfStep_inj In Out\<cdot>h\<cdot>sb \<rightleftharpoons> sb)\<cdot>b)) = Out"
-      by simp 
+    proof -
+      have "True \<and> ubDom\<cdot>(spfStep_inj In Out\<cdot>h\<cdot>b \<rightleftharpoons> b) = Out"
+        by (metis \<open>ubDom\<cdot>(b::'a stream\<^sup>\<Omega>) = (In::channel set)\<close> assms spfStep_inj_out_dom ubclDom_ubundle_def)
+      then show ?thesis
+        by (simp add: \<open>ubDom\<cdot>(b::'a stream\<^sup>\<Omega>) = (In::channel set)\<close>)
+    qed
   next
     fix b2::"'a SB"
     assume "ubDom\<cdot>b2 = In"
@@ -517,99 +648,80 @@ lemma spfStep_inj_inner_well[simp]:"ufWell(\<Lambda> sb. (ubDom\<cdot>sb = In) \
       by (simp add: domIff)
 qed
 
-lemma spfStep_cont[simp]:"cont(\<lambda> h. Abs_ufun(\<Lambda> sb. (ubDom\<cdot>sb = In) \<leadsto> spfStep_inj In Out\<cdot>h\<cdot>sb \<rightleftharpoons> sb))"
+lemma spfStep_cont[simp]:assumes "finite In" 
+  shows "cont(\<lambda> h. Abs_ufun(\<Lambda> sb. (ubDom\<cdot>sb = In) \<leadsto> spfStep_inj In Out\<cdot>h\<cdot>sb \<rightleftharpoons> sb))"
 proof(rule Cont.contI2)
-  show "monofun (\<lambda>h::'a sbElem \<Rightarrow> ('a stream\<^sup>\<Omega>) ufun. Abs_cufun (\<lambda>sb::'a stream\<^sup>\<Omega>. (ubDom\<cdot>sb = In)\<leadsto>spfStep_inj In Out\<cdot>h\<cdot>sb \<rightleftharpoons> sb))"
-  proof(rule monofunI)
-    fix x y::"'a sbElem \<Rightarrow> ('a stream\<^sup>\<Omega>) ufun"
-    assume a1:"x \<sqsubseteq> y"
-    show "Abs_cufun (\<lambda>sb. (ubDom\<cdot>sb = In)\<leadsto>spfStep_inj In Out\<cdot>x\<cdot>sb \<rightleftharpoons> sb) \<sqsubseteq> Abs_cufun (\<lambda>sb. (ubDom\<cdot>sb = In)\<leadsto>spfStep_inj In Out\<cdot>y\<cdot>sb \<rightleftharpoons> sb)"
-      apply(simp add: below_ufun_def below_cfun_def below_fun_def, auto)
-      by (meson a1 cfun_below_iff monofun_cfun_arg some_below spf_pref_eq_2)
+  show "monofun
+     (\<lambda>h::'a sbElem \<Rightarrow> ('a stream\<^sup>\<Omega>) ufun.
+         Abs_cufun (\<lambda>sb::'a stream\<^sup>\<Omega>. (ubDom\<cdot>sb = In)\<leadsto>spfStep_inj In Out\<cdot>h\<cdot>sb \<rightleftharpoons> sb))"
+    apply (rule monofunI)
+    apply(simp add: below_ufun_def below_cfun_def below_fun_def, auto)
+    apply (simp add: assms rep_abs_cufun)
+  proof -
+    fix x :: "'a sbElem \<Rightarrow> ('a stream\<^sup>\<Omega>) ufun" and y :: "'a sbElem \<Rightarrow> ('a stream\<^sup>\<Omega>) ufun" and xa :: "'a stream\<^sup>\<Omega>"
+    assume "\<forall>xa xb. Rep_cufun (x xa) xb \<sqsubseteq> Rep_cufun (y xa) xb"
+    then have "x \<sqsubseteq> y"
+      by (simp add: below_fun_def below_ufun_def cfun_below_iff)
+    moreover
+    { assume "Rep_cufun (spfStep_inj In Out\<cdot>y\<cdot>xa) xa \<noteq> Rep_cufun (spfStep_inj In Out\<cdot>x\<cdot>xa) xa \<and> x \<sqsubseteq> y"
+      then have "ubDom\<cdot>xa = In \<longrightarrow> Some (spfStep_inj In Out\<cdot>x\<cdot>xa \<rightleftharpoons> xa) \<sqsubseteq> Some (spfStep_inj In Out\<cdot>y\<cdot>xa \<rightleftharpoons> xa)"
+        by (metis (no_types) below_option_def below_ufun_def cfun_below_iff monofun_cfun_arg some_below) }
+    ultimately show "ubDom\<cdot>xa = In \<longrightarrow> Some (spfStep_inj In Out\<cdot>x\<cdot>xa \<rightleftharpoons> xa) \<sqsubseteq> Some (spfStep_inj In Out\<cdot>y\<cdot>xa \<rightleftharpoons> xa)"
+      by fastforce
   qed
 next
-  fix Y::"nat \<Rightarrow> 'a sbElem \<Rightarrow> ('a stream\<^sup>\<Omega>) ufun"
-  assume a1:"chain Y"
-  assume a2:"chain (\<lambda>i::nat. Abs_cufun (\<lambda>sb::'a stream\<^sup>\<Omega>. (ubDom\<cdot>sb = In)\<leadsto>spfStep_inj In Out\<cdot>(Y i)\<cdot>sb \<rightleftharpoons> sb))"
-  have h1_0:"\<And>sb. (spfStep_inj In Out\<cdot>(\<Squnion>i. Y i)\<cdot>sb \<rightleftharpoons> sb) = (\<Squnion>i. spfStep_inj In Out\<cdot>(Y i)\<cdot>sb \<rightleftharpoons> sb)"
-    apply(subst contlub_cfun_arg, simp add: a1)
-    apply(subst contlub_cfun_fun)
-    using a1 apply auto[1]
-    apply(rule spfapply_lub)
-    using a1 by auto[1]
-    have h0_2:"\<forall>sb. ((ubDom\<cdot>sb = In)\<leadsto>\<Squnion>i. spfStep_inj In Out\<cdot>(Y i)\<cdot>sb \<rightleftharpoons> sb) = (\<Squnion>i. (ubDom\<cdot>sb = In)\<leadsto>spfStep_inj In Out\<cdot>(Y i)\<cdot>sb \<rightleftharpoons> sb)"
-  proof(auto)
-    fix sb::"'a stream\<^sup>\<Omega>"
-    assume a11: "In = ubDom\<cdot>sb"  
-    have h0_21:"((ubDom\<cdot>sb = In)\<leadsto>(\<Squnion>i. spfStep_inj In Out\<cdot>(Y i)\<cdot>sb \<rightleftharpoons> sb)) = (\<Squnion>i. (ubDom\<cdot>sb = In)\<leadsto>spfStep_inj In Out\<cdot>(Y i)\<cdot>sb \<rightleftharpoons> sb)"
-    proof(cases "ubDom\<cdot>sb = In")
-      case True
-      then show ?thesis 
-        apply auto
-        apply(rule some_lub_chain_eq2)
-        by (meson a1 monofun_cfun_arg monofun_cfun_fun po_class.chain_def spf_pref_eq_2)
-    next
-      case False
-      then show ?thesis 
-        by simp
-    qed
-    show"Some (\<Squnion>i. (spfStep_inj (ubDom\<cdot>sb) Out\<cdot>(Y i)\<cdot>sb) \<rightleftharpoons> sb) = (\<Squnion>i. Some ((spfStep_inj (ubDom\<cdot>sb) Out\<cdot>(Y i)\<cdot>sb) \<rightleftharpoons> sb))"
-      using a11 h0_21 by auto
-  qed 
-  have cont_lub2:"cont (\<lambda>x. \<Squnion>i. (ubDom\<cdot>x = In)\<leadsto>spfStep_inj In Out\<cdot>(Y i)\<cdot>x \<rightleftharpoons> x)"
-    apply(rule cont2cont_lub)
-    apply(rule chainI)
-    apply (smt a1 cont_pref_eq1I eq_imp_below monofun_cfun_fun po_class.chain_def some_below spf_pref_eq_2)
-    by simp  
-  have ufWell:"ufWell (\<Lambda> x. \<Squnion>i::nat. Rep_cufun (Abs_cufun (\<lambda>sb::'a stream\<^sup>\<Omega>. (ubDom\<cdot>sb = In)\<leadsto>spfStep_inj In Out\<cdot>(Y i)\<cdot>sb \<rightleftharpoons> sb)) x)"
-  apply(subst rep_abs_cufun, simp, simp)
-  proof(rule ufwellI)
-    fix b:: "'a stream\<^sup>\<Omega>"    
-    assume "b \<in> dom (Rep_cfun (\<Lambda> (x::'a stream\<^sup>\<Omega>). \<Squnion>i::nat. (ubDom\<cdot>x = In)\<leadsto>spfStep_inj In Out\<cdot>(Y i)\<cdot>x \<rightleftharpoons> x))"
-    hence b_def:" b \<in> dom (\<lambda> x. \<Squnion>i. (ubDom\<cdot>x = In) \<leadsto> spfStep_inj In Out\<cdot>(Y i)\<cdot>x \<rightleftharpoons> x)"
-      using cont_lub2 by auto
-    thus "ubDom\<cdot>b = In"
-      by (metis (no_types, lifting) domIff h0_2)
-    thus "ubDom\<cdot>Rep_cfun (\<Lambda> x. \<Squnion>i. (ubDom\<cdot>x = In)\<leadsto>spfStep_inj In Out\<cdot>(Y i)\<cdot>x \<rightleftharpoons> x)\<rightharpoonup>b = Out"
-      apply(subst beta_cfun,subst cont_lub2, simp,simp)
-      by (smt h0_2 h1_0 lub_eq option.sel spfStep_inj_out_dom)
-  next
-    fix b2::"'a stream\<^sup>\<Omega>"
-    assume "ubDom\<cdot>b2 = In"
-    thus "b2 \<in> dom (Rep_cfun (\<Lambda> x. \<Squnion>i. (ubDom\<cdot>x = In)\<leadsto>spfStep_inj In Out\<cdot>(Y i)\<cdot>x \<rightleftharpoons> x))"
-    proof -
-      show ?thesis
-        by (metis (lifting) Abs_cfun_inverse2 \<open>ubDom\<cdot>b2 = In\<close> cont_lub2 domIff h0_2 option.distinct(1))
-    qed
-  qed
-  have h1:"(\<lambda>sb. (ubDom\<cdot>sb = In)\<leadsto>spfStep_inj In Out\<cdot>(\<Squnion>i. Y i)\<cdot>sb \<rightleftharpoons> sb) \<sqsubseteq> Rep_cufun (\<Squnion>i. Abs_cufun (\<lambda>sb. (ubDom\<cdot>sb = In)\<leadsto>spfStep_inj In Out\<cdot>(Y i)\<cdot>sb \<rightleftharpoons> sb))"
-    apply(subst h1_0, subst h0_2)
-    apply(subst lub_ufun)
-    apply (simp add: a2)
-    apply(subst lub_cfun)
-    using a2 rep_ufun_chain apply blast
-    apply(subst rep_abs_cufun)
-    apply(subst rep_abs_cufun, simp,simp)
-    apply(simp_all only: ufWell cont_lub2)
-    by simp
-  show " Abs_cufun (\<lambda>sb. (ubDom\<cdot>sb = In)\<leadsto>spfStep_inj In Out\<cdot>(\<Squnion>i. Y i)\<cdot>sb \<rightleftharpoons> sb) \<sqsubseteq>
+  fix Y ::"nat \<Rightarrow> 'a sbElem \<Rightarrow> ('a stream\<^sup>\<Omega>) ufun"
+  assume y_chain: "chain Y"
+  assume cufun_chain: "chain (\<lambda>i::nat. Abs_cufun (\<lambda>sb::'a stream\<^sup>\<Omega>. (ubDom\<cdot>sb = In)\<leadsto>spfStep_inj In Out\<cdot>(Y i)\<cdot>sb \<rightleftharpoons> sb))"
+  have dom_L: "ufDom\<cdot>
+    (Abs_cufun
+      (\<lambda>sb::'a stream\<^sup>\<Omega>.
+          (ubDom\<cdot>sb = In)\<leadsto>spfStep_inj In Out\<cdot>(\<Squnion>i::nat. Y i)\<cdot>sb \<rightleftharpoons> sb)) = In"
+    apply (fold ubclDom_ubundle_def)
+    apply (rule ufun_ufdom_abs)
+     apply (simp add: ubclDom_ubundle_def)
+    by (simp add: assms ubclDom_ubundle_def)
+  have dom_R: "ufDom\<cdot>
+    (\<Squnion>i::nat.
+        Abs_cufun
+         (\<lambda>sb::'a stream\<^sup>\<Omega>. (ubDom\<cdot>sb = In)\<leadsto>spfStep_inj In Out\<cdot>(Y i)\<cdot>sb \<rightleftharpoons> sb)) = In"
+    apply (fold ubclDom_ubundle_def)
+    apply (subst ufdom_lub_eq)
+     apply (simp add: cufun_chain ubclDom_ubundle_def)
+    apply (rule ufun_ufdom_abs)
+    apply (simp add: ubclDom_ubundle_def)
+    by (simp add: assms ubclDom_ubundle_def)
+  show "Abs_cufun (\<lambda>sb::'a stream\<^sup>\<Omega>. (ubDom\<cdot>sb = In)\<leadsto>spfStep_inj In Out\<cdot>(\<Squnion>i::nat. Y i)\<cdot>sb \<rightleftharpoons> sb) \<sqsubseteq>
        (\<Squnion>i::nat. Abs_cufun (\<lambda>sb::'a stream\<^sup>\<Omega>. (ubDom\<cdot>sb = In)\<leadsto>spfStep_inj In Out\<cdot>(Y i)\<cdot>sb \<rightleftharpoons> sb))"
-    by(simp add: below_ufun_def below_cfun_def h1)
+    apply (rule ufun_belowI)
+     apply (simp_all add: dom_L dom_R)
+     apply (simp_all add: rep_abs_cufun assms)
+    apply (fold ubclDom_ubundle_def)
+    apply simp
+    apply (simp add: rep_cufun_lub_apply ubclDom_ubundle_def cufun_chain)
+    apply (simp add: rep_abs_cufun assms ubclDom_ubundle_def)
+    by (simp add: contlub_cfun_arg contlub_cfun_fun spfapply_lub y_chain)
 qed
      
 
-lemma spfstep_dom[simp]:"ufDom\<cdot>(spfStep cIn cOut\<cdot>f) = cIn"
-  sorry
+lemma spfstep_dom[simp]:assumes "finite cIn" shows "ufDom\<cdot>(spfStep cIn cOut\<cdot>f) = cIn"
+  apply (simp add: spfStep_def assms)
+  apply (fold ubclDom_ubundle_def)
+  apply (rule ufun_ufdom_abs)
+  by (simp_all add: assms ubclDom_ubundle_def)
     
-lemma spfstep_ran [simp]:"ufRan\<cdot>(spfStep cIn cOut\<cdot>f) = cOut"
-  sorry
+lemma spfstep_ran [simp]:assumes "finite cIn" shows "ufRan\<cdot>(spfStep cIn cOut\<cdot>f) = cOut"
+  apply (subst ufran_least)
+  apply (simp add: assms)
+  apply (simp add: spfStep_def assms)
+  by (metis ubclDom_ubundle_def ubcldom_least_cs)
     
     
-lemma spfstep_inj_dom[simp]:"ufDom\<cdot>(spfStep_inj cIn cOut\<cdot>f\<cdot>sb) = cIn"
-  sorry
+lemma spfstep_inj_dom[simp]:assumes "finite cIn" shows "ufDom\<cdot>(spfStep_inj cIn cOut\<cdot>f\<cdot>sb) = cIn"
+  by (simp add:  assms spfStep_inj_def)
     
-lemma spfstep_inj_ran [simp]:"ufRan\<cdot>(spfStep_inj cIn cOut\<cdot>f\<cdot>sb) = cOut"
-  sorry
+lemma spfstep_inj_ran [simp]:assumes "finite cIn" shows "ufRan\<cdot>(spfStep_inj cIn cOut\<cdot>f\<cdot>sb) = cOut"
+  by (simp add:  assms spfStep_inj_def)
     
 lemma test2:"ubDom\<cdot>sb \<noteq> In \<Longrightarrow> (ufRestrict In Out\<cdot>spf \<rightleftharpoons> sb) = the None"
   apply(simp add: ufRestrict_def)
@@ -620,13 +732,11 @@ lemma test2_2:"ubDom\<cdot>sb \<noteq> In \<Longrightarrow> (ufLeast In Out \<ri
   by (simp add: ubclDom_ubundle_def)
     
   
-lemma spfStep_2_spfStep_inj: "spfStep In Out\<cdot>h \<rightleftharpoons> sb = spfStep_inj In Out\<cdot>h\<cdot>sb \<rightleftharpoons> sb"
+lemma spfStep_2_spfStep_inj: assumes "finite In" shows "spfStep In Out\<cdot>h \<rightleftharpoons> sb = spfStep_inj In Out\<cdot>h\<cdot>sb \<rightleftharpoons> sb"
   apply(rule ub_eq)
-   apply (metis (no_types, lifting) option.exhaust_sel spfstep_dom spfstep_inj_dom spfstep_inj_ran
-      spfstep_ran ubclDom_ubundle_def ufdom_2ufundom ufran_2_ubcldom2)
-  apply(simp add: spfStep_def spfStep_inj_def, auto)
-  using test2 test2_2 by fastforce+
-    
+   apply (metis (no_types, hide_lams) assms not_None_eq spfstep_dom spfstep_inj_dom 
+      spfstep_inj_ran spfstep_ran ubclDom_ubundle_def ufdom_2ufundom ufran_2_ubcldom2)
+  by (simp add: assms spfStep_def spfStep_inj_def test2_2)
 (* lemma spfstep_insert  *)
 
     
