UFun.thy
@@ -288,6 +288,28 @@ lemma rep_ufun_well [simp]:  "ufWell (Rep_ufun s)"
 lemma rep_cufun_cont [simp]: "cont Rep_cufun"
   by simp
 
+lemma rep_cufun_lub: assumes "chain Y" shows "Rep_cufun (Lub Y) = (\<Squnion> i. Rep_cufun( Y i))"
+proof -
+have f1: "\<forall>F f. \<not> F <<| (f::'a \<Rightarrow> 'a option) \<or> lub F = f"
+  by (meson lub_eqI)
+  have "range (\<lambda>n. Rep_cufun (Y n)) <<| Rep_cufun (Lub Y)"
+    using assms cont_def by force
+then show ?thesis
+    using f1 by presburger
+qed
+
+lemma rep_cufun_lub_apply: assumes "chain Y" shows "(Lub Y) \<rightleftharpoons> x = (\<Squnion> i. ( Y i)  \<rightleftharpoons> x)"
+proof -
+  have f1: "chain (\<lambda>n. Rep_ufun (Y n))"
+    using assms rep_ufun_chain by blast
+  then have f2: "chain (\<lambda>n. Rep_cufun (Y n) x)"
+    using ch2ch_Rep_cfunL by blast
+  have "\<forall>f. \<not> chain f \<or> (Lub f::'a \<rightarrow> 'a option) = Abs_cfun (\<Squnion>n. Rep_cfun (f n))"
+    using cfun.lub_cfun by blast
+  then show ?thesis
+    using f2 f1 by (metis (no_types) assms contlub_cfun_fun eta_cfun lub_eq op_the_lub rep_cufun_lub)
+qed
+
 (* Rep_cufun produces a ufwell function  *)
 lemma rep_cufun_well [simp]: "ufWell (Abs_cfun (Rep_cufun x))"
   by (simp add: Cfun.cfun.Rep_cfun_inverse)
